LambdaS5/coq/LjsPrettyRulesAux.v
@@ -3,13 +3,12 @@ Set Implicit Arguments.
 Require Import Utils.
 Require Import LjsShared.
 Require Import LjsSyntax.
+Require Import LjsSyntaxAux.
 Require Import LjsPrettyInterm.
 Require Import LjsPrettyRules.
 Require Import LjsStore.
 Require Import LjsCommon.
 Require Import LjsValues.
-Require Import LjsOperators.
-Require Import LjsMonads.
 Require Import JsNumber.
 Import List.ListNotations.
 
@@ -34,6 +33,87 @@ Proof.
     unfolds in Hout;
     inverts Hred; tryfalse; injects; jauto.
 Qed.
+
+Fixpoint pure_expr_pred c st e v : Prop :=
+    match e with
+    | expr_undefined => v = value_undefined
+    | expr_null => v = value_null
+    | expr_empty => v = value_empty
+    | expr_bool b => v = value_bool b
+    | expr_string s => v = value_string s
+    | expr_number n => v = value_number n
+    | expr_lambda is e => v = add_closure c None is e
+    | expr_id s => binds c s v 
+    | expr_if e1 e2 e3 => exists b, pure_expr_pred c st e1 (value_bool b) /\ 
+        (b /\ pure_expr_pred c st e2 v \/ ~b /\ pure_expr_pred c st e3 v) 
+    | expr_let s e1 e2 => exists v', pure_expr_pred c st e1 v' /\ pure_expr_pred (c \(s := v')) st e2 v
+    | expr_seq e1 e2 => pure_expr_pred c st e2 v
+    | expr_jseq e1 e2 => exists v1 v2, pure_expr_pred c st e1 v1 /\ pure_expr_pred c st e2 v2 /\
+        v = overwrite_value_if_empty v1 v2
+    | expr_op1 op e => exists v', pure_expr_pred c st e v' /\ eval_unary_op op st v' v
+    | expr_op2 op e1 e2 => exists v1 v2, pure_expr_pred c st e1 v1 /\ pure_expr_pred c st e2 v2 /\
+        eval_binary_op op st v1 v2 v
+    | expr_get_attr pa e1 e2 => exists ptr obj s attrs, 
+        pure_expr_pred c st e1 (value_object ptr) /\ 
+        pure_expr_pred c st e2 (value_string s) /\
+        binds st ptr obj /\ binds (object_properties obj) s attrs /\
+        attributes_pattr_readable attrs pa /\ v = get_attributes_pattr attrs pa
+    | expr_get_obj_attr oa e => exists ptr obj,
+        pure_expr_pred c st e (value_object ptr) /\
+        binds st ptr obj /\
+        v = get_object_oattr obj oa
+    | _ => False
+    end.
+
+Fixpoint bool_expr_pred c st e : Prop :=
+    match e with
+    | expr_bool true => True
+    | expr_bool false => False
+    | expr_if e1 e2 e3 => 
+        bool_expr_pred c st e1 /\ bool_expr_pred c st e2 \/ ~bool_expr_pred c st e1 /\ bool_expr_pred c st e3
+    | expr_let s e1 e2 =>
+        exists v, pure_expr_pred c st e1 v /\ bool_expr_pred (c \(s := v)) st e2
+    | expr_op1 unary_op_is_primitive e => exists v, pure_expr_pred c st e v /\ is_primitive v
+    | expr_op1 unary_op_is_closure e => exists v, pure_expr_pred c st e v /\ is_closure v
+    | expr_op1 unary_op_is_object e => exists v, pure_expr_pred c st e v /\ is_object v
+    | expr_op1 unary_op_prim_to_bool e => exists v, pure_expr_pred c st e v /\ value_to_bool_cast v
+    | expr_op1 unary_op_not e => ~bool_expr_pred c st e
+    | expr_op2 binary_op_stx_eq e1 e2 => 
+        exists v1 v2, pure_expr_pred c st e1 v1 /\ pure_expr_pred c st e2 v2 /\ stx_eq v1 v2
+    | expr_op2 binary_op_same_value e1 e2 => 
+        exists v1 v2, pure_expr_pred c st e1 v1 /\ pure_expr_pred c st e2 v2 /\ same_value v1 v2
+    | expr_op2 binary_op_has_property e1 e2 => 
+        exists ptr obj s, pure_expr_pred c st e1 (value_object ptr) /\ pure_expr_pred c st e2 (value_string s) /\
+        binds st ptr obj /\ exists att, object_property_is st obj s (Some att)
+    | expr_op2 binary_op_has_own_property e1 e2 => 
+        exists ptr obj s, pure_expr_pred c st e1 (value_object ptr) /\ pure_expr_pred c st e2 (value_string s) /\
+        binds st ptr obj /\ index (object_properties obj) s
+    | expr_op2 binary_op_has_internal e1 e2 => 
+        exists ptr obj s, pure_expr_pred c st e1 (value_object ptr) /\ pure_expr_pred c st e2 (value_string s) /\
+        binds st ptr obj /\ index (object_internal obj) s
+    | expr_op2 binary_op_is_accessor e1 e2 => 
+        exists ptr obj s att, pure_expr_pred c st e1 (value_object ptr) /\ pure_expr_pred c st e2 (value_string s) /\
+        binds st ptr obj /\ object_property_is st obj s (Some att) /\ is_accessor att
+    | expr_op2 binary_op_string_lt e1 e2 => 
+        exists s1 s2, pure_expr_pred c st e1 (value_string s1) /\ pure_expr_pred c st e2 (value_string s2) /\
+        string_lt s1 s2
+    | expr_op2 binary_op_locale_compare e1 e2 => 
+        exists s1 s2, pure_expr_pred c st e1 (value_string s1) /\ pure_expr_pred c st e2 (value_string s2) /\
+        string_lt s1 s2
+    | expr_op2 binary_op_lt e1 e2 => 
+        exists n1 n2, pure_expr_pred c st e1 (value_number n1) /\ pure_expr_pred c st e2 (value_number n2) /\
+        num_lt n1 n2
+    | expr_op2 binary_op_gt e1 e2 => 
+        exists n1 n2, pure_expr_pred c st e1 (value_number n1) /\ pure_expr_pred c st e2 (value_number n2) /\
+        num_gt n1 n2
+    | expr_op2 binary_op_le e1 e2 => 
+        exists n1 n2, pure_expr_pred c st e1 (value_number n1) /\ pure_expr_pred c st e2 (value_number n2) /\
+        num_le n1 n2
+    | expr_op2 binary_op_ge e1 e2 => 
+        exists n1 n2, pure_expr_pred c st e1 (value_number n1) /\ pure_expr_pred c st e2 (value_number n2) /\
+        num_ge n1 n2
+    | _ => False
+    end.
 
 Lemma object_property_is_deterministic : forall st obj name oattr oattr',
     object_property_is st obj name oattr -> object_property_is st obj name oattr' -> oattr = oattr'.
@@ -83,6 +163,339 @@ Proof.
     repeat binds_determine; try reflexivity.
     rewrite H1 in *. injects. reflexivity. 
     lets X : object_property_is_deterministic H1 H5. injects. reflexivity.
+Qed.
+
+Ltac false_abort := 
+    match goal with
+    | H : abort _ |- _ => solve [invert H as H; invert H]
+    end.
+
+Lemma pure_expr_lemma : forall c st st' e r,
+    pure_expr e ->
+    red_expr c st e (out_ter st' r) ->
+    st = st' /\ exists v,
+    r = res_value v /\ pure_expr_pred c st e v.
+Proof.
+    introv Hpe Hred.
+    inductions Hpe gen c st st' r Hred;
+    inverts Hred as Hr1 Hr2; simpl; jauto.
+    (* if *)
+    forwards Hx : out_red_ter Hr2. reflexivity. destruct_hyp Hx.
+    specializes IHHpe1 Hr1. destruct_hyp IHHpe1.
+    inverts Hr2 as Hr2.
+    specializes IHHpe2 Hr2. destruct_hyp IHHpe2.
+    jauto.
+    specializes IHHpe3 Hr2. destruct_hyp IHHpe3.
+    jauto.
+    false_abort.
+    (* seq *)
+    forwards Hx : out_red_ter Hr2. reflexivity. destruct_hyp Hx.
+    inverts Hr2 as Hr2.
+    specializes IHHpe1 Hr1. destruct_hyp IHHpe1.
+    specializes IHHpe2 Hr2. destruct_hyp IHHpe2.
+    jauto.
+    specializes IHHpe1 Hr1. destruct_hyp IHHpe1.
+    false_abort.
+    (* jseq *)
+    forwards Hx : out_red_ter Hr2. reflexivity. destruct_hyp Hx.
+    specializes IHHpe1 Hr1. destruct_hyp IHHpe1.
+    inverts Hr2 as Hr2 Hr3; [idtac | false_abort].
+    forwards Hx : out_red_ter Hr3. reflexivity. destruct_hyp Hx.
+    specializes IHHpe2 Hr2. destruct_hyp IHHpe2.
+    inverts Hr3.
+    jauto.
+    (* let *)
+    forwards Hx : out_red_ter Hr2. reflexivity. destruct_hyp Hx.
+    specializes IHHpe1 Hr1. destruct_hyp IHHpe1.
+    inverts Hr2 as Hr2; [idtac | false_abort].
+    specializes IHHpe2 Hr2. destruct_hyp IHHpe2.
+    jauto.
+    (* unary *)
+    forwards Hx : out_red_ter Hr2. reflexivity. destruct_hyp Hx.
+    specializes IHHpe Hr1. destruct_hyp IHHpe.
+    inverts Hr2 as Hr2; [idtac | false_abort].
+    jauto.
+    (* binary *)    
+    forwards Hx : out_red_ter Hr2. reflexivity. destruct_hyp Hx.
+    specializes IHHpe1 Hr1. destruct_hyp IHHpe1.
+    inverts Hr2 as Hr2 Hr3; [idtac | false_abort].
+    forwards Hx : out_red_ter Hr3. reflexivity. destruct_hyp Hx.
+    specializes IHHpe2 Hr2. destruct_hyp IHHpe2.
+    inverts Hr3 as Hr3; [idtac | false_abort].
+    jauto.
+    (* get_attr *)
+    inverts Hr1 as Hr1 Hr2.
+    forwards Hx : out_red_ter Hr2. reflexivity. destruct_hyp Hx.
+    specializes IHHpe1 Hr1. destruct_hyp IHHpe1.
+    inverts Hr2 as Hr2; [idtac | false_abort].
+    inverts Hr2 as Hr2 Hr3.
+    forwards Hx : out_red_ter Hr3. reflexivity. destruct_hyp Hx.
+    specializes IHHpe2 Hr2. destruct_hyp IHHpe2.
+    inverts Hr3 as Hr3; [idtac | false_abort].
+    inverts Hr3 as Hr3. inverts Hr3 as Hr3.
+    jauto.
+    (* get_obj_attr *)
+    forwards Hx : out_red_ter Hr2. reflexivity. destruct_hyp Hx.
+    specializes IHHpe Hr1. destruct_hyp IHHpe.
+    inverts Hr2 as Hr2; [idtac | false_abort].
+    jauto.
+Qed.
+
+Lemma pure_expr_pred_deterministic : forall c st e v v',
+    pure_expr_pred c st e v -> pure_expr_pred c st e v' -> v = v'.
+Proof.
+    introv Hpe1 Hpe2.
+    inductions e gen c st Hpe1 Hpe2; simpls; substs; repeat binds_determine; try reflexivity; tryfalse.
+    (* get_attr *)
+    destruct Hpe1 as (?ptr&?obj&?s&?attrs&Hpe1&Hpf1&Hb1&Hbp1&Hre1&Heq1).
+    destruct Hpe2 as (?ptr&?obj&?s&?attrs&Hpe2&Hpf2&Hb2&Hbp2&Hre2&Heq2).
+    specializes IHe1 Hpe1 Hpe2.
+    specializes IHe2 Hpf1 Hpf2.
+    repeat injects. substs. repeat binds_determine.
+    reflexivity.
+    (* get_obj_attr *)
+    destruct Hpe1 as (?ptr&?obj&Hpe1&Hb1&Heq1).
+    destruct Hpe2 as (?ptr&?obj&Hpe2&Hb2&Heq2).
+    specializes IHe Hpe1 Hpe2.
+    repeat injects. substs. repeat binds_determine.
+    reflexivity.
+    (* unary *)
+    destruct Hpe1 as (?v&Hpe1&Hun1).
+    destruct Hpe2 as (?v&Hpe2&Hun2).
+    specializes IHe Hpe1 Hpe2. substs.
+    applys eval_unary_op_deterministic Hun1 Hun2.
+    (* binary *)
+    destruct Hpe1 as (?v&?v&Hpe1&Hpf1&Hun1).
+    destruct Hpe2 as (?v&?v&Hpe2&Hpf2&Hun2).
+    specializes IHe1 Hpe1 Hpe2.
+    specializes IHe2 Hpf1 Hpf2. substs.
+    applys eval_binary_op_deterministic Hun1 Hun2.
+    (* if *)
+    destruct Hpe1 as (b1&Hpe1&Hcond1).
+    destruct Hpe2 as (b2&Hpe2&Hcond2).
+    specializes IHe1 Hpe1 Hpe2.
+    injects.
+    destruct b2;
+    rew_refl in Hcond1; rew_refl in Hcond2;
+    rew_logic in Hcond1; rew_logic in Hcond2.
+    specializes IHe2 Hcond1 Hcond2.
+    specializes IHe3 Hcond1 Hcond2.
+    (* seq *)
+    eauto.
+    (* jseq *)
+    destruct Hpe1 as (?v&?v&Hpe1&Hpf1&Heq1).
+    destruct Hpe2 as (?v&?v&Hpe2&Hpf2&Heq2).
+    specializes IHe1 Hpe1 Hpe2.
+    specializes IHe2 Hpf1 Hpf2.
+    substs. reflexivity.
+    (* let *)
+    destruct Hpe1 as (?v&Hpe1&Hpf1).
+    destruct Hpe2 as (?v&Hpe2&Hpf2).
+    specializes IHe1 Hpe1 Hpe2. substs.
+    specializes IHe2 Hpf1 Hpf2.
+Qed.
+
+Lemma pure_expr_pred_op1_lemma : forall P c st e v,
+    pure_expr_pred c st e v ->
+    P v = exists v', pure_expr_pred c st e v' /\ P v'.
+Proof.
+    introv Hpur.
+    rew_logic. split. jauto.
+    introv (v'&Hpur'&Hp').
+    lets Heq : pure_expr_pred_deterministic Hpur Hpur'. substs. 
+    assumption.
+Qed.
+
+Lemma pure_expr_pred_op2_lemma : forall P c st e1 e2 v1 v2,
+    pure_expr_pred c st e1 v1 ->
+    pure_expr_pred c st e2 v2 ->
+    P v1 v2 = exists v1' v2', pure_expr_pred c st e1 v1' /\ pure_expr_pred c st e2 v2' /\ P v1' v2'.
+Proof.
+    introv Hpur1 Hpur2.
+    rew_logic. split. jauto.
+    introv (v1'&v2'&Hpur1'&Hpur2'&Hp').
+    lets Heq1 : pure_expr_pred_deterministic Hpur1 Hpur1'. 
+    lets Heq2 : pure_expr_pred_deterministic Hpur2 Hpur2'. 
+    substs. 
+    assumption.
+Qed.
+
+Lemma pure_expr_pred_op2_number_lemma : forall P c st e1 e2 n1 n2,
+    pure_expr_pred c st e1 (value_number n1) ->
+    pure_expr_pred c st e2 (value_number n2) ->
+    P n1 n2 = exists n1' n2', 
+        pure_expr_pred c st e1 (value_number n1') /\ pure_expr_pred c st e2 (value_number n2') /\ P n1' n2'.
+Proof.
+    introv Hpur1 Hpur2.
+    rew_logic. split. jauto.
+    introv (v1'&v2'&Hpur1'&Hpur2'&Hp').
+    lets Heq1 : pure_expr_pred_deterministic Hpur1 Hpur1'. 
+    lets Heq2 : pure_expr_pred_deterministic Hpur2 Hpur2'. 
+    repeat injects. 
+    assumption.
+Qed.
+
+Lemma pure_expr_pred_op2_string_lemma : forall P c st e1 e2 s1 s2,
+    pure_expr_pred c st e1 (value_string s1) ->
+    pure_expr_pred c st e2 (value_string s2) ->
+    P s1 s2 = exists s1' s2', 
+        pure_expr_pred c st e1 (value_string s1') /\ pure_expr_pred c st e2 (value_string s2') /\ P s1' s2'.
+Proof.
+    introv Hpur1 Hpur2.
+    rew_logic. split. jauto.
+    introv (v1'&v2'&Hpur1'&Hpur2'&Hp').
+    lets Heq1 : pure_expr_pred_deterministic Hpur1 Hpur1'. 
+    lets Heq2 : pure_expr_pred_deterministic Hpur2 Hpur2'. 
+    repeat injects. 
+    assumption.
+Qed.
+
+Lemma pure_expr_pred_op2_object_string_lemma : forall P c st e1 e2 obj ptr s,
+    pure_expr_pred c st e1 (value_object ptr) ->
+    pure_expr_pred c st e2 (value_string s) ->
+    binds st ptr obj ->
+    P obj s = exists ptr' obj' s', 
+        pure_expr_pred c st e1 (value_object ptr') /\ pure_expr_pred c st e2 (value_string s') /\ 
+        binds st ptr' obj' /\ P obj' s'.
+Proof.
+    introv Hpur1 Hpur2 Hbinds.
+    rew_logic. split. jauto.
+    introv (obj'&ptr'&s'&Hpur1'&Hpur2'&Hbinds'&Hp').
+    lets Heq1 : pure_expr_pred_deterministic Hpur1 Hpur1'. 
+    lets Heq2 : pure_expr_pred_deterministic Hpur2 Hpur2'. 
+    repeat injects. 
+    binds_determine.
+    assumption.
+Qed.
+
+Lemma pure_expr_pred_op2_object_attrs_string_lemma : forall P c st e1 e2 obj ptr att s,
+    pure_expr_pred c st e1 (value_object ptr) ->
+    pure_expr_pred c st e2 (value_string s) ->
+    binds st ptr obj ->
+    object_property_is st obj s (Some att) ->
+    P obj s att = exists ptr' obj' s' att', 
+        pure_expr_pred c st e1 (value_object ptr') /\ pure_expr_pred c st e2 (value_string s') /\ 
+        binds st ptr' obj' /\ object_property_is st obj' s' (Some att') /\ P obj' s' att'.
+Proof.
+    introv Hpur1 Hpur2 Hbinds Hprop.
+    rew_logic. split. jauto.
+    introv (obj'&ptr'&s'&att'&Hpur1'&Hpur2'&Hbinds'&Hprop'&Hp').
+    lets Heq1 : pure_expr_pred_deterministic Hpur1 Hpur1'. 
+    lets Heq2 : pure_expr_pred_deterministic Hpur2 Hpur2'. 
+    repeat injects. 
+    binds_determine.
+    lets Heq3 : object_property_is_deterministic Hprop Hprop'.
+    injects.
+    assumption.
+Qed.
+
+Lemma bool_red_expr_lemma : forall c st st' e r,
+    bool_expr e ->
+    red_expr c st e (out_ter st' r) ->
+    st = st' /\ r = res_value (value_bool (isTrue (bool_expr_pred c st e))).
+Proof.
+    introv Hpe Hred.
+    inductions Hpe gen c st st' r Hred;
+    inverts Hred as Hr1 Hr2; simpl; jauto.
+    (* bool *)
+    cases_if; rew_refl; jauto.
+    (* if *) 
+    forwards Hx : out_red_ter Hr2. reflexivity. destruct_hyp Hx.
+    specializes IHHpe1 Hr1. destruct_hyp IHHpe1.
+    rew_unreflect.
+    cases_isTrue in * as Eq;
+    rew_bool;
+    (inverts Hr2 as Hr2; [idtac | false_abort]).
+    specializes IHHpe2 Hr2. destruct_hyp IHHpe2. jauto.
+    specializes IHHpe3 Hr2. destruct_hyp IHHpe3. jauto.
+    (* let *)
+    forwards Hx : out_red_ter Hr2. reflexivity. destruct_hyp Hx.
+    forwards Hpur : pure_expr_lemma Hr1. assumption. destruct_hyp Hpur.
+    inverts Hr2 as Hr2; [idtac | false_abort].
+    specializes IHHpe Hr2. destruct_hyp IHHpe. 
+    forwards Heq : pure_expr_pred_op1_lemma (fun v => bool_expr_pred (c\(s:=v)) st' e2). eassumption.
+    rewrite Heq. jauto. 
+    (* not *)
+    forwards Hx : out_red_ter Hr2. reflexivity. destruct_hyp Hx.
+    specializes IHHpe Hr1. destruct_hyp IHHpe.
+    inverts Hr2 as Hr2; [idtac | false_abort].
+    inverts Hr2. rew_refl. jauto.
+    (* op1 *)
+    forwards Hx : out_red_ter Hr2. reflexivity. destruct_hyp Hx.
+    forwards Hpur : pure_expr_lemma Hr1. assumption. destruct_hyp Hpur. clear Hr1.
+    inverts Hr2 as Hr2; [idtac | false_abort].
+    destruct op; tryfalse; inverts Hr2; try false_invert.
+    (* is_primitive *)
+    forwards Heq : pure_expr_pred_op1_lemma is_primitive. eassumption. 
+    rewrite decide_spec. rewrite Heq. jauto. 
+    (* is_closure *)
+    forwards Heq : pure_expr_pred_op1_lemma is_closure. eassumption. 
+    rewrite decide_spec. rewrite Heq. jauto. 
+    (* is_object *)
+    forwards Heq : pure_expr_pred_op1_lemma is_object. eassumption. 
+    rewrite decide_spec. rewrite Heq. jauto. 
+    (* prim_to_bool *)
+    forwards Heq : pure_expr_pred_op1_lemma value_to_bool_cast. eassumption. 
+    rewrite <- (isTrue_istrue (value_to_bool_cast v)).
+    rewrite Heq. jauto.
+    (* op2 *)
+    forwards Hx : out_red_ter Hr2. reflexivity. destruct_hyp Hx.
+    forwards Hpur : pure_expr_lemma Hr1. assumption. destruct_hyp Hpur. clear Hr1.
+    inverts Hr2 as Hr2 Hr3; [idtac | false_abort].
+    forwards Hx : out_red_ter Hr3. reflexivity. destruct_hyp Hx.
+    forwards Hpur : pure_expr_lemma Hr2. assumption. destruct_hyp Hpur. clear Hr2.
+    inverts Hr3 as Hr3; [idtac | false_abort].
+    destruct op; tryfalse; inverts Hr3 as Hr3; try false_invert.
+    (* lt *)
+    inverts Hr3.
+    forwards Heq : pure_expr_pred_op2_number_lemma num_lt Hpur2 Hpur3.
+    rewrite <- (isTrue_istrue (num_lt n1 n2)).
+    rewrite Heq. jauto.
+    (* le *)
+    inverts Hr3.
+    forwards Heq : pure_expr_pred_op2_number_lemma num_le Hpur2 Hpur3.
+    rewrite <- (isTrue_istrue (num_le n1 n2)).
+    rewrite Heq. jauto.
+    (* gt *)
+    inverts Hr3.
+    forwards Heq : pure_expr_pred_op2_number_lemma num_gt Hpur2 Hpur3.
+    rewrite <- (isTrue_istrue (num_gt n1 n2)).
+    rewrite Heq. jauto.
+    (* ge *)
+    inverts Hr3.
+    forwards Heq : pure_expr_pred_op2_number_lemma num_ge Hpur2 Hpur3.
+    rewrite <- (isTrue_istrue (num_ge n1 n2)).
+    rewrite Heq. jauto.
+    (* stx_eq *) 
+    forwards Heq : pure_expr_pred_op2_lemma stx_eq Hpur2 Hpur3.
+    rewrite decide_spec. rewrite Heq. jauto.
+    (* same_value *)
+    forwards Heq : pure_expr_pred_op2_lemma same_value Hpur2 Hpur3.
+    rewrite decide_spec. rewrite Heq. jauto.
+    (* object_has_property *)
+    forwards Heq : pure_expr_pred_op2_object_string_lemma
+        (fun obj s => exists att, object_property_is st' obj s (Some att)) Hpur2 Hpur3 Hr3.
+    rewrite Heq. jauto.
+    (* has_own_property *)
+    forwards Heq : pure_expr_pred_op2_object_string_lemma
+        (fun obj s => index (object_properties obj) s) Hpur2 Hpur3 Hr3.
+    rewrite decide_spec. rewrite Heq. jauto.
+    (* has_internal *)
+    forwards Heq : pure_expr_pred_op2_object_string_lemma
+        (fun obj s => index (object_internal obj) s) Hpur2 Hpur3 Hr3.
+    rewrite decide_spec. rewrite Heq. jauto.
+    (* is_accessor *)
+    forwards Heq : pure_expr_pred_op2_object_attrs_string_lemma
+        (fun obj s attrs => is_accessor attrs) Hpur2 Hpur3 Hr3. eassumption.
+    rewrite decide_spec. rewrite Heq. jauto.
+    (* string_lt *)
+    forwards Heq : pure_expr_pred_op2_string_lemma string_lt Hpur2 Hpur3.
+    rewrite <- (isTrue_istrue (string_lt s1 s2)).
+    rewrite Heq. jauto.
+    (* locale_compare *)
+    forwards Heq : pure_expr_pred_op2_string_lemma string_lt Hpur2 Hpur3.
+    rewrite <- (isTrue_istrue (string_lt s1 s2)).
+    rewrite Heq. jauto.
 Qed.
 
 Module Export Tactics.
