LambdaS5/coq/LjsSyntaxAux.v
@@ -15,19 +15,220 @@ Proof.
     intros. apply (prove_Inhab value_undefined).
 Qed.
 
-Inductive pure_expr : ctx -> expr -> Prop :=
-| pure_expr_empty : forall c, pure_expr c expr_empty
-| pure_expr_null : forall c, pure_expr c expr_null
-| pure_expr_undefined : forall c, pure_expr c expr_undefined
-| pure_expr_string : forall c s, pure_expr c (expr_string s)
-| pure_expr_number : forall c n, pure_expr c (expr_number n)
-| pure_expr_true : forall c, pure_expr c expr_true
-| pure_expr_false : forall c, pure_expr c expr_false
-| pure_expr_id : forall c i, index c i -> pure_expr c (expr_id i)
-| pure_expr_if : forall c e1 e2 e3, 
-    pure_expr c e1 -> pure_expr c e2 -> pure_expr c e3 -> 
-    pure_expr c (expr_if e1 e2 e3)
-| pure_expr_seq : forall c e1 e2, 
-    pure_expr c e1 -> pure_expr c e2 ->
-    pure_expr c (expr_seq e1 e2)
+Inductive type :=
+| type_empty
+| type_undefined
+| type_null
+| type_bool
+| type_number
+| type_string
+| type_object
+| type_closure
 .
+
+Definition value_type v :=
+    match v with
+    | value_empty => type_empty
+    | value_undefined => type_undefined
+    | value_null => type_null
+    | value_bool _ => type_bool
+    | value_number _ => type_number
+    | value_string _ => type_string
+    | value_object _ => type_object
+    | value_closure _ => type_closure
+    end.
+
+Inductive unary_op_type : unary_op -> type -> type -> Prop := 
+(* debugging operators *)
+| unary_op_type_print : forall t, unary_op_type unary_op_print t type_undefined
+| unary_op_type_pretty : forall t, unary_op_type unary_op_pretty t type_undefined
+(* string operators *)
+| unary_op_type_strlen : unary_op_type unary_op_strlen type_string type_number
+| unary_op_type_ascii_ntoc : unary_op_type unary_op_ascii_ntoc type_number type_string
+| unary_op_type_ascii_cton : unary_op_type unary_op_ascii_cton type_string type_number
+(* type testing operators *)
+| unary_op_type_typeof : forall t, unary_op_type unary_op_typeof t type_string
+| unary_op_type_is_primitive : forall t, unary_op_type unary_op_is_primitive t type_bool
+| unary_op_type_is_closure : forall t, unary_op_type unary_op_is_closure t type_bool
+| unary_op_type_is_object : forall t, unary_op_type unary_op_is_object t type_bool
+(* number operators *)
+| unary_op_type_abs : unary_op_type unary_op_abs type_number type_number
+| unary_op_type_floor : unary_op_type unary_op_floor type_number type_number
+| unary_op_type_neg : unary_op_type unary_op_neg type_number type_number
+(* conversion operators *)
+| unary_op_type_prim_to_str : forall t, unary_op_type unary_op_prim_to_bool t type_string
+| unary_op_type_prim_to_num : forall t, unary_op_type unary_op_prim_to_bool t type_number
+| unary_op_type_prim_to_bool : forall t, unary_op_type unary_op_prim_to_bool t type_bool
+(* logic operators *)
+| unary_op_type_not : unary_op_type unary_op_not type_bool type_bool
+(* int operators *)
+| unary_op_type_bnot : unary_op_type unary_op_bnot type_number type_number
+| unary_op_type_to_int32 : unary_op_type unary_op_to_int32 type_number type_number
+.
+
+Definition unary_op_ret_type op :=
+    match op with 
+    (* debugging operators *)
+    | unary_op_print 
+    | unary_op_pretty => type_undefined
+    (* string operators *)
+    | unary_op_strlen => type_number
+    | unary_op_ascii_ntoc => type_string
+    | unary_op_ascii_cton => type_number
+    (* type testing operators *)
+    | unary_op_typeof => type_string
+    | unary_op_is_primitive 
+    | unary_op_is_closure 
+    | unary_op_is_object => type_bool
+    (* number operators *)
+    | unary_op_abs 
+    | unary_op_floor 
+    | unary_op_neg => type_number
+    (* conversion operators *)
+    | unary_op_prim_to_str => type_string
+    | unary_op_prim_to_num => type_number
+    | unary_op_prim_to_bool => type_bool
+    (* logic operators *)
+    | unary_op_not => type_bool
+    (* int operators *)
+    | unary_op_bnot => type_number
+    | unary_op_to_int32 => type_number
+    (* undefined operators *)
+    | _ => type_undefined
+    end.
+
+Inductive binary_op_type : binary_op -> type -> type -> type -> Prop := 
+(* arithmetic operators *)
+| binary_op_type_add : binary_op_type binary_op_add type_number type_number type_number
+| binary_op_type_sub : binary_op_type binary_op_sub type_number type_number type_number
+| binary_op_type_mul : binary_op_type binary_op_mul type_number type_number type_number
+| binary_op_type_div : binary_op_type binary_op_div type_number type_number type_number
+| binary_op_type_mod : binary_op_type binary_op_mod type_number type_number type_number
+(* comparison operators *)
+| binary_op_type_lt : binary_op_type binary_op_lt type_number type_number type_bool
+| binary_op_type_le : binary_op_type binary_op_le type_number type_number type_bool
+| binary_op_type_gt : binary_op_type binary_op_gt type_number type_number type_bool
+| binary_op_type_ge : binary_op_type binary_op_ge type_number type_number type_bool
+(* string comparison operators *)
+| binary_op_type_string_lt : binary_op_type binary_op_string_lt type_string type_string type_bool
+| binary_op_type_locale_compare : binary_op_type binary_op_locale_compare type_string type_string type_bool
+(* equality operators *)
+| binary_op_type_stx_eq : forall t1 t2, binary_op_type binary_op_stx_eq t1 t2 type_bool
+| binary_op_type_same_value : forall t1 t2, binary_op_type binary_op_same_value t1 t2 type_bool
+(* object inspection operators *)
+| binary_op_type_has_property : binary_op_type binary_op_has_property type_object type_string type_bool
+| binary_op_type_has_own_property : binary_op_type binary_op_has_own_property type_object type_string type_bool
+| binary_op_type_has_internal : binary_op_type binary_op_has_internal type_object type_string type_bool
+| binary_op_type_is_accessor : binary_op_type binary_op_is_accessor type_object type_string type_bool
+(* string operators *)
+| binary_op_type_string_plus : binary_op_type binary_op_string_plus type_string type_string type_string
+| binary_op_type_char_at : binary_op_type binary_op_char_at type_string type_number type_string
+(* int operators (bitwise and shifts) *)
+| binary_op_type_band : binary_op_type binary_op_band type_number type_number type_number
+| binary_op_type_bor : binary_op_type binary_op_bor type_number type_number type_number
+| binary_op_type_bxor : binary_op_type binary_op_bxor type_number type_number type_number
+| binary_op_type_shiftl : binary_op_type binary_op_shiftl type_number type_number type_number
+| binary_op_type_shiftr : binary_op_type binary_op_shiftr type_number type_number type_number
+| binary_op_type_zfshiftr : binary_op_type binary_op_zfshiftr type_number type_number type_number
+.
+
+Definition binary_op_ret_type op := 
+    match op with
+    (* arithmetic operators *)
+    | binary_op_add 
+    | binary_op_sub 
+    | binary_op_mul 
+    | binary_op_div 
+    | binary_op_mod => type_number
+    (* comparison operators *)
+    | binary_op_lt 
+    | binary_op_le 
+    | binary_op_gt 
+    | binary_op_ge 
+    (* string comparison operators *)
+    | binary_op_string_lt 
+    | binary_op_locale_compare 
+    (* equality operators *)
+    | binary_op_stx_eq 
+    | binary_op_same_value 
+    (* object inspection operators *)
+    | binary_op_has_property 
+    | binary_op_has_own_property 
+    | binary_op_has_internal 
+    | binary_op_is_accessor => type_bool
+    (* string operators *)
+    | binary_op_string_plus 
+    | binary_op_char_at => type_string
+    (* int operators (bitwise and shifts) *)
+    | binary_op_band 
+    | binary_op_bor
+    | binary_op_bxor 
+    | binary_op_shiftl 
+    | binary_op_shiftr 
+    | binary_op_zfshiftr => type_number
+    (* undefined operators *)
+    | _ => type_undefined
+    end.
+
+Inductive pure_expr : expr -> Prop :=
+| pure_expr_empty : pure_expr expr_empty
+| pure_expr_null : pure_expr expr_null
+| pure_expr_undefined : pure_expr expr_undefined
+| pure_expr_string : forall s, pure_expr (expr_string s)
+| pure_expr_number : forall n, pure_expr (expr_number n)
+| pure_expr_bool : forall b, pure_expr (expr_bool b)
+| pure_expr_lambda : forall is e, pure_expr (expr_lambda is e)
+| pure_expr_id : forall i, pure_expr (expr_id i)
+| pure_expr_if : forall e1 e2 e3, 
+    pure_expr e1 -> pure_expr e2 -> pure_expr e3 -> 
+    pure_expr (expr_if e1 e2 e3)
+| pure_expr_seq : forall e1 e2, 
+    pure_expr e1 -> pure_expr e2 ->
+    pure_expr (expr_seq e1 e2)
+| pure_expr_jseq : forall e1 e2, 
+    pure_expr e1 -> pure_expr e2 ->
+    pure_expr (expr_jseq e1 e2)
+| pure_expr_let : forall s e1 e2, 
+    pure_expr e1 -> pure_expr e2 ->
+    pure_expr (expr_let s e1 e2)
+| pure_expr_op1 : forall op e, 
+    pure_expr e ->
+    pure_expr (expr_op1 op e)
+| pure_expr_op2 : forall op e1 e2, 
+    pure_expr e1 -> pure_expr e2 ->
+    pure_expr (expr_op2 op e1 e2)
+| pure_expr_get_attr : forall pa e1 e2,
+    pure_expr e1 -> pure_expr e2 ->
+    pure_expr (expr_get_attr pa e1 e2)
+| pure_expr_get_oattr : forall oa e,
+    pure_expr e ->
+    pure_expr (expr_get_obj_attr oa e)
+.
+
+Inductive bool_expr : expr -> Prop :=
+| bool_expr_bool : forall b, bool_expr (expr_bool b)
+| bool_expr_if : forall e1 e2 e3,
+    bool_expr e1 -> bool_expr e2 -> bool_expr e3 ->
+    bool_expr (expr_if e1 e2 e3)
+| bool_expr_let : forall s e1 e2,
+    pure_expr e1 -> bool_expr e2 -> 
+    bool_expr (expr_let s e1 e2)
+| bool_expr_not : forall e,
+    bool_expr e ->
+    bool_expr (expr_op1 unary_op_not e)
+| bool_expr_op1 : forall op e,
+    unary_op_ret_type op = type_bool ->
+    op <> unary_op_not ->
+    pure_expr e ->
+    bool_expr (expr_op1 op e)
+| bool_expr_op2 : forall op e1 e2,
+    binary_op_ret_type op = type_bool ->
+    pure_expr e1 ->
+    pure_expr e2 ->
+    bool_expr (expr_op2 op e1 e2)
+.
+
+Create HintDb ljs discriminated.
+
+Hint Constructors pure_expr : ljs.
+Hint Constructors bool_expr : ljs.
